prefix dcm: <http://purl.org/dc/dcmitype/>
prefix dct: <http://purl.org/dc/terms/>
prefix foaf: <http://xmlns.com/foaf/0.1/>
prefix owl: <http://www.w3.org/2002/07/owl#>
prefix rdf: <http://www.w3.org/1999/02/22-rdf-syntax-ns#>
prefix rdfs: <http://www.w3.org/2000/01/rdf-schema#>
prefix skos: <http://www.w3.org/2004/02/skos/core#>
prefix standard: <https://data.rijksfinancien.nl/xmlns/id/standard/>
prefix status: <http://purl.org/adms/status/>
prefix vann: <http://purl.org/vocab/vann/>
prefix void: <http://rdfs.org/ns/void#>
prefix xml: <http://www.w3.org/XML/1998/namespace#model/def/> 
prefix xmlns: <http://www.w3.org/2000/xmlns/> 
prefix xsd: <http://www.w3.org/2001/XMLSchema#>

  xmlns:
    a
      owl:Ontology,
      void:Dataset;
    dct:created '2024-02-19'^^xsd:date;
    dct:creator
      'Flores Bakker';
    dct:language 'iso639-1:en';
    dct:license 'http://creativecommons.org/licenses/by/4.0'^^xsd:anyURI;
    dct:publisher <https://rijksfinancien.nl>;
    dct:status status:UnderDevelopment;
    dct:subject 'xmlns'@en;
    dct:title 'XMLNS Ontology'@en;
    dct:source <https://github.com/floresbakker/xmlnsvoc>;
    dct:abstract "The XMLNS Core Ontology provides a formal representation of XML Namespace declarations. It defines classes and properties to describe XML Namespace attributes and their usage within XML documents."@en;
    dct:description "The XMLNS Ontology formalizes XML Namespace declarations, offering a structured representation of namespace attributes and their significance within XML documents. It includes definitions for essential concepts such as xmlns:xsi, xmlns:rdf, xmlns:xlink, xmlns:dc, xmlns:cc, etc. The ontology serves as a reference for understanding and working with XML Namespace declarations within the context of RDF-based applications."@en;
    foaf:depiction 'https://www.rijksfinancien.nl/themes/custom/indicia_theme/files/logo-rijksoverheid.svg'^^xsd:anyURI;
    foaf:homepage 'https://www.rijksfinancien.nl/'^^xsd:anyURI;
    owl:imports
      dct:,
      owl:,
      rdf:,
      rdfs:,
      skos:;
    owl:versionInfo '0.1.0';
    vann:preferredNamespacePrefix 'xmlns';
    vann:preferredNamespaceUri 'http://www.w3.org/2000/xmlns/';
    void:uriRegexPattern '^http://www.w3.org/2000/xmlns/';
    void:uriSpace 'http://www.w3.org/2000/xmlns/'^^xsd:anyURI.

  standard:xmlns
    a dct:Standard;
    dct:created '2024-02-19'^^xsd:date;
    dct:source 'https://www.w3.org/TR/xml-names11/'^^xsd:anyURI;
    skos:prefLabel 'Namespaces in XML 1.1 (Second Edition)'@en.

### Attribute

  xmlns:xsi 
    a owl:DatatypeProperty;
    xml:key 'xsi';
    rdfs:domain xml:Element;
    rdfs:range xsd:string;
    rdfs:subPropertyOf xml:attribute;
    skos:definition "The 'xsi' attribute is used to specify the XML Schema Instance namespace within an XML document. It associates elements and attributes with XML Schema definitions."@en;
    skos:prefLabel 'the xsi attribute'@en;
    rdfs:isDefinedBy xmlns:.

  xmlns:rdf
    a owl:DatatypeProperty;
    xml:key 'rdf';
    rdfs:domain xml:Element;
    rdfs:range xsd:string;
    rdfs:subPropertyOf xml:attribute;
    skos:definition "The 'rdf' attribute is used to specify the RDF namespace within an XML document. It associates elements and attributes with RDF resources and statements."@en;
    skos:prefLabel 'the rdf attribute'@en;
    rdfs:isDefinedBy xmlns:.

  xmlns:xlink 
    a owl:DatatypeProperty;
    xml:key 'xlink';
    rdfs:domain xml:Element;
    rdfs:range xsd:string;
    rdfs:subPropertyOf xml:attribute;
    skos:definition "The 'xlink' attribute is used to specify the XLink namespace within an XML document. It associates elements and attributes with XLink resources and links."@en;
    skos:prefLabel 'the xlink attribute'@en;
    rdfs:isDefinedBy xmlns:.

  xmlns:dc 
    a owl:DatatypeProperty;
    xml:key 'dc';
    rdfs:domain xml:Element;
    rdfs:range xsd:string;
    rdfs:subPropertyOf xml:attribute;
    skos:definition "The 'dc' attribute is used to specify the Dublin Core namespace within an XML document. It associates elements and attributes with Dublin Core metadata terms."@en;
    skos:prefLabel 'the dc attribute'@en;
    rdfs:isDefinedBy xmlns:.

  xmlns:cc
    a owl:DatatypeProperty;
    xml:key 'cc';
    rdfs:domain xml:Element;
    rdfs:range xsd:string;
    rdfs:subPropertyOf xml:attribute;
    skos:definition "The 'cc' attribute is used to specify the Creative Commons namespace within an XML document. It associates elements and attributes with Creative Commons licenses and metadata."@en;
    skos:prefLabel 'the cc attribute'@en;
    rdfs:isDefinedBy xmlns:.

