# Generic prefixes
prefix dcm: <http://purl.org/dc/dcmitype/>
prefix dct: <http://purl.org/dc/terms/>
prefix foaf: <http://xmlns.com/foaf/0.1/>
prefix owl: <http://www.w3.org/2002/07/owl#>
prefix rdf: <http://www.w3.org/1999/02/22-rdf-syntax-ns#>
prefix rdfs: <http://www.w3.org/2000/01/rdf-schema#>
prefix skos: <http://www.w3.org/2004/02/skos/core#>
prefix status: <http://purl.org/adms/status/>
prefix vann: <http://purl.org/vocab/vann/>
prefix void: <http://rdfs.org/ns/void#>
prefix xml: <http://www.w3.org/XML/model/def/> 
prefix xsd: <http://www.w3.org/2001/XMLSchema#>

# XSI prefixes
prefix section: <http://www.w3.org/2001/XMLSchema-instance/id/section/>
prefix standard: <http://www.w3.org/2001/XMLSchema-instance/id/standard/>
prefix xsi: <http://www.w3.org/2001/XMLSchema-instance/model/def/>

xsi: {
  xsi:
    a
      owl:Ontology,
      void:Dataset;
    dct:created '2023-10-29'^^xsd:date;
    dct:creator
      'Flores Bakker';
    dct:language 'iso639-1:en';
    dct:license 'http://creativecommons.org/licenses/by/4.0'^^xsd:anyURI;
    dct:publisher <https://rijksfinancien.nl>;
    dct:status status:UnderDevelopment;
    dct:subject 'xsi'@en;
    dct:title 'XSI Ontology'@en;
    dct:source <https://github.com/floresbakker/xsivoc>;
    dct:abstract "The XSI (XML Schema Instance) Core Ontology provides a formal representation of concepts related to XML Schema instance documents. It defines terms and relationships necessary for describing XML documents and their validation using XML Schema."@en;
    dct:description "The XSI (XML Schema Instance) Ontology captures the essential elements and attributes associated with XML Schema instance documents. It formalizes concepts such as schema location and data types specified in XML documents, particularly for validation purposes using XML Schema definitions (XSD). This ontology aims to enhance interoperability and understanding of XML-based data exchange and validation processes."@en;
    foaf:depiction 'https://www.rijksfinancien.nl/themes/custom/indicia_theme/files/logo-rijksoverheid.svg'^^xsd:anyURI;
    foaf:homepage 'https://www.rijksfinancien.nl/'^^xsd:anyURI;
    owl:imports
      dct:,
      owl:,
      rdf:,
      rdfs:,
      skos:;
    owl:versionInfo '0.1.0';
    vann:preferredNamespacePrefix 'xsi';
    vann:preferredNamespaceUri 'http://www.w3.org/XML/model/def/';
    void:uriRegexPattern '^http://www.w3.org/XML/model/def/';
    void:uriSpace 'http://www.w3.org/XML/model/def/'^^xsd:anyURI.

  standard:xsi
    a dct:Standard;
    dct:created '2024-02-19'^^xsd:date;
    dct:source 'https://www.w3.org/TR/xmlschema-1/'^^xsd:anyURI;
    skos:prefLabel 'XML Schema Part 1: Structures Second Edition'@en.

  section:2.6.1
    a dcm:Text;
    dct:isPartOf standard:xlink;
    dct:source 'https://www.w3.org/TR/xmlschema-1/#xsi_type'^^xsd:anyURI;
    skos:prefLabel 'ยง 2.6.1 xsi:type'@en;
    rdfs:isDefinedBy xsi:.

  section:2.6.2
    a dcm:Text;
    dct:isPartOf standard:xlink;
    dct:source 'https://www.w3.org/TR/xmlschema-1/#xsi_nil'^^xsd:anyURI;
    skos:prefLabel 'ยง 2.6.2 xsi:nil'@en;
    rdfs:isDefinedBy xsi:.

  section:2.6.3
    a dcm:Text;
    dct:isPartOf standard:xlink;
    dct:source 'https://www.w3.org/TR/xmlschema-1/#xsi_schemaLocation'^^xsd:anyURI;
    skos:prefLabel 'ยง 2.6.3 xsi:schemaLocation, xsi:noNamespaceSchemaLocation'@en;
    rdfs:isDefinedBy xsi:.

### Classes ###

  xsi:Attribute
    rdf:type owl:Class;
    rdfs:subClassOf xml:Attribute;
    dct:conformsTo section:AttributesAndSyntax;
    skos:definition """An XSI attribute is used to provide information related to XML Schema validation within an XML document. Such an attribute allows XML documents to declare how they relate to XML Schemas, specify the data types of elements, and control schema validation behavior."""@en;
    skos:prefLabel 'attribute'@en;
    rdfs:isDefinedBy xsi:.

### Properties ###

  xsi:nil
    a owl:DatatypeProperty;
    dct:conformsTo section:2.6.2;
    xml:key 'nil';
    rdfs:domain xml:Element;
    rdfs:range xsd:string;
    rdfs:subPropertyOf xml:attribute;
    rdf:type xsi:Attribute;
    skos:definition "The xsi:nil attribute indicates whether an element has a nil value. When the xsi:nil attribute is set to 'true', it signifies that the element has no value. This attribute is typically used in XML Schema instance documents to represent null or empty values for elements defined in XML Schema."@en;
    skos:prefLabel 'the nil attribute'@en;
    rdfs:isDefinedBy xsi:.

  xsi:schemaLocation
    a owl:DatatypeProperty;
    dct:conformsTo section:2.6.3;
    xml:key 'schemaLocation';
    rdfs:domain xml:Element;
    rdfs:range xsd:string;
    rdfs:subPropertyOf xml:attribute;
    rdf:type xsi:Attribute;    
    skos:definition "The 'schemaLocation' attribute is used in XML documents associated with XML Schema validation. It specifies the location of the XML Schema definition (XSD) that describes the structure and constraints of elements in the document."@en;
    skos:prefLabel 'the schemaLocation attribute'@en;
    rdfs:isDefinedBy xsi:.

  xsi:type
    a owl:DatatypeProperty;
    dct:conformsTo section:2.6.1;
    xml:key 'type';
    rdfs:domain xml:Element;
    rdfs:range xsd:string;
    rdfs:subPropertyOf xml:attribute;
    rdf:type xsi:Attribute;    
    skos:definition "The 'type' attribute is used in XML documents associated with XML Schema validation. It specifies the data type of an element or an attribute in accordance with the XML Schema definition (XSD)."@en;
    skos:prefLabel 'the type attribute'@en;
    rdfs:isDefinedBy xsi:.

}